slight cleanup

examples/layeredeffects/Common.fst
@@ -2,6 +2,12 @@ module Common
 
 (* Common lemmas and constructions for layered effects examples. *)
 
+let coerce #a #b (x:a{a == b}) : b = x
+
+let unreachable (#a:Type u#aa) () : Pure a (requires False) (ensures (fun _ -> False)) =
+  coerce #(raise_t string) #a (raise_val "whatever")
+
+
 let elim_pure #a #wp ($f : unit -> PURE a wp) p
  : Pure a (requires (wp p)) (ensures (fun r -> p r))
  //: PURE a (fun p' -> wp p /\ (forall r. p r ==> p' r))
